Weidenbach_Book/DPLL_NOT.thy
@@ -128,7 +128,7 @@ proof -
     hence "F \<Turnstile>as CNot (image_mset uminus ?C)"
        unfolding M CNot_def true_annots_def by (auto simp add: L lits_of_def)
   ultimately show ?thesis
-    using M' \<open>D \<in># snd ?S\<close> L by auto
+    using M' \<open>D \<in># snd ?S\<close> L by force
 qed
 
 lemma backtrack_is_backjump':
@@ -196,14 +196,14 @@ qed
 end
 
 sublocale dpll_with_backtrack \<subseteq> dpll_with_backjumping_ops fst snd "\<lambda>L (M, N). (L # M, N)"
-  "\<lambda>(M, N). (tl M, N)" "\<lambda>C (M, N). (M, {#C#} + N)" "\<lambda>C (M, N). (M, remove_mset N C)" "\<lambda>_. True"
+  "\<lambda>(M, N). (tl M, N)" "\<lambda>C (M, N). (M, {#C#} + N)" "\<lambda>C (M, N). (M, remove_mset N C)" "\<lambda>_ _. True"
   "\<lambda>(M, N). no_dup M \<and> all_decomposition_implies_m N (get_all_marked_decomposition M)"
   "(\<lambda>_ _ S T. backtrack S T)"
   by unfold_locales (metis (mono_tags, lifting) dpll_with_backtrack.backtrack_is_backjump''
    dpll_with_backtrack.can_do_bt_step prod.case_eq_if comp_apply)
 
 sublocale dpll_with_backtrack \<subseteq> dpll_with_backjumping fst snd "\<lambda>L (M, N). (L # M, N)"
-  "\<lambda>(M, N). (tl M, N)" "\<lambda>C (M, N). (M, {#C#} + N)" "\<lambda>C (M, N). (M, remove_mset N C)" "\<lambda>_. True"
+  "\<lambda>(M, N). (tl M, N)" "\<lambda>C (M, N). (M, {#C#} + N)" "\<lambda>C (M, N). (M, remove_mset N C)" "\<lambda>_ _. True"
   "\<lambda>(M, N). no_dup M \<and> all_decomposition_implies_m N (get_all_marked_decomposition M)"
   "(\<lambda>_ _ S T. backtrack S T)"
   apply unfold_locales
@@ -212,14 +212,14 @@ sublocale dpll_with_backtrack \<subseteq> dpll_with_backjumping fst snd "\<lambd
 
 sublocale dpll_with_backtrack \<subseteq> conflict_driven_clause_learning_ops
   fst snd "\<lambda>L (M, N). (L # M, N)"
-  "\<lambda>(M, N). (tl M, N)" "\<lambda>C (M, N). (M, {#C#} + N)" "\<lambda>C (M, N). (M, remove_mset N C)" "\<lambda>_. True"
+  "\<lambda>(M, N). (tl M, N)" "\<lambda>C (M, N). (M, {#C#} + N)" "\<lambda>C (M, N). (M, remove_mset N C)" "\<lambda>_ _. True"
   "\<lambda>(M, N). no_dup M \<and> all_decomposition_implies_m N (get_all_marked_decomposition M)"
   "(\<lambda>_ _ S T. backtrack S T)" "\<lambda>_ _. False" "\<lambda>_ _. False"
   by unfold_locales
 
 sublocale dpll_with_backtrack \<subseteq> conflict_driven_clause_learning
   fst snd "\<lambda>L (M, N). (L # M, N)"
-  "\<lambda>(M, N). (tl M, N)" "\<lambda>C (M, N). (M, {#C#} + N)" "\<lambda>C (M, N). (M, remove_mset N C)" "\<lambda>_. True"
+  "\<lambda>(M, N). (tl M, N)" "\<lambda>C (M, N). (M, {#C#} + N)" "\<lambda>C (M, N). (M, remove_mset N C)" "\<lambda>_ _. True"
   "\<lambda>(M, N). no_dup M \<and> all_decomposition_implies_m N (get_all_marked_decomposition M)"
   "(\<lambda>_ _ S T. backtrack S T)" "\<lambda>_ _. False" "\<lambda>_ _. False"
   apply unfold_locales
